Claude splits up AddAux

bignums.dfy
@@ -384,38 +384,315 @@ lemma Thirteen()
   }
 }
 
+predicate AddAuxPred(x: string, y: string, oldSb: string, sb: string, oldI: int,
+                     oldJ: int, i:int, j:int, carry:nat, bitX:nat, bitY:nat, digit:nat, sum:nat, oldCarry:nat)
+{
+  ValidBitString(sb) &&
+  ValidBitString(x) &&
+  ValidBitString(y) &&
+  ValidBitString(oldSb) &&
+  0 <= carry <= 1 &&
+  i <= |x| - 1 && j <= |y| - 1 &&
+  oldI <= |x| - 1 && oldJ <= |y| - 1 &&
+  i >= -1 &&
+  j >= -1 &&
+  (oldI >= 0 ==> i == oldI - 1) &&
+  (oldJ >= 0 ==> j == oldJ - 1) &&
+  (oldI < 0 ==> i == oldI) &&
+  (oldJ < 0 ==> j == oldJ) &&
+  (oldI >= 0 ==> (bitX == if x[oldI] == '1' then 1 else 0)) &&
+  (oldJ >= 0 ==> (bitY == if y[oldJ] == '1' then 1 else 0)) &&
+  (oldI < 0 ==> bitX == 0) &&
+  (oldJ < 0 ==> bitY == 0) &&
+  |oldSb| == |sb| - 1 &&
+  sum == bitX + bitY + oldCarry &&
+  digit == sum % 2 &&
+  carry == sum / 2 &&
+  (if digit == 1 then ['1'] + oldSb else ['0'] + oldSb) == sb
+}
 
-// I pulled this code out of `Add` in the hope that Dafny would avoid timeouts
-// if it was in the narrower context of a lemma. Unfortunately that didn't
-// fix the timeouts, but `Add` is easier to read with this long calculation removed.
-// Annoyingly if you remove {:isolate_assertions}, this lemma sometimes times out.
-// So really I need to go over it again to reduce brittleness, as in
-// https://dafny.org/blog/2023/12/01/avoiding-verification-brittleness/
-// I didn't check whether some of the intermediate steps can be taken out
-lemma {:isolate_assertions} AddAux(x: string, y: string, oldSb: string, sb: string, oldI: int,
-                                   oldJ: int, i:int, j:int, carry:nat, bitX:nat, bitY:nat, digit:nat, sum:nat, oldCarry:nat)
-  requires ValidBitString(sb)
-  requires ValidBitString(x)
-  requires ValidBitString(y)
-  requires ValidBitString(oldSb)
-  requires 0 <= carry <= 1
-  requires i <= |x| - 1 && j <= |y| - 1
-  requires oldI <= |x| - 1 && oldJ <= |y| - 1
-  requires i >= -1
-  requires j >= -1
-  requires oldI >= 0 ==> i == oldI - 1
-  requires oldJ >= 0 ==> j == oldJ - 1
-  requires oldI < 0 ==> i == oldI
-  requires oldJ < 0 ==> j == oldJ
-  requires oldI >= 0 ==> (bitX == if x[oldI] == '1' then 1 else 0)
-  requires oldJ >= 0 ==> (bitY == if y[oldJ] == '1' then 1 else 0)
-  requires oldI < 0 ==> bitX == 0
-  requires oldJ < 0 ==> bitY == 0
-  requires |oldSb| == |sb| - 1
-  requires sum == bitX + bitY + oldCarry
-  requires digit == sum % 2
-  requires carry == sum / 2
-  requires (if digit == 1 then ['1'] + oldSb else ['0'] + oldSb) == sb
+// Lemma 1: Apply BitStringDecomposition for both numbers
+lemma AddAux1(x: string, y: string, oldSb: string, sb: string, oldI: int,
+              oldJ: int, i:int, j:int, carry:nat, bitX:nat, bitY:nat, digit:nat, sum:nat, oldCarry:nat)
+  requires AddAuxPred(x, y, oldSb, sb, oldI, oldJ, i, j, carry, bitX, bitY, digit, sum, oldCarry)
+  ensures Str2Int(oldSb) +
+          (oldCarry * Pow2(|oldSb|)) +
+          (if oldI >= 0 then Str2Int(x[0..oldI+1]) * Pow2(|oldSb|) else 0) +
+          (if oldJ >= 0 then Str2Int(y[0..oldJ+1]) * Pow2(|oldSb|) else 0) ==
+          Str2Int(oldSb) +
+          (oldCarry * Pow2(|oldSb|)) +
+          (if oldI >= 0 then (Str2Int(x[0..oldI]) * 2 + bitX) * Pow2(|oldSb|) else 0) +
+          (if oldJ >= 0 then (Str2Int(y[0..oldJ]) * 2 + bitY) * Pow2(|oldSb|) else 0)
+{
+  BitStringDecomposition(x, oldI);
+  BitStringDecomposition(y, oldJ);
+}
+
+// Lemma 2: Distribute Pow2(|oldSb|) in the third term
+lemma AddAux2(x: string, y: string, oldSb: string, sb: string, oldI: int,
+              oldJ: int, i:int, j:int, carry:nat, bitX:nat, bitY:nat, digit:nat, sum:nat, oldCarry:nat)
+  requires AddAuxPred(x, y, oldSb, sb, oldI, oldJ, i, j, carry, bitX, bitY, digit, sum, oldCarry)
+  ensures Str2Int(oldSb) +
+          (oldCarry * Pow2(|oldSb|)) +
+          (if oldI >= 0 then (Str2Int(x[0..oldI]) * 2 + bitX) * Pow2(|oldSb|) else 0) +
+          (if oldJ >= 0 then (Str2Int(y[0..oldJ]) * 2 + bitY) * Pow2(|oldSb|) else 0) ==
+          Str2Int(oldSb) +
+          (oldCarry * Pow2(|oldSb|)) +
+          (if oldI >= 0 then (Str2Int(x[0..oldI]) * 2) * Pow2(|oldSb|) + bitX * Pow2(|oldSb|) else 0) +
+          (if oldJ >= 0 then (Str2Int(y[0..oldJ]) * 2 + bitY) * Pow2(|oldSb|) else 0)
+{
+  if oldI >= 0 {
+    var A := Str2Int(x[0..oldI]);
+    var B := bitX;
+    var C := Pow2(|oldSb|);
+    Rearrange(A, B, C);
+  }
+}
+
+
+// Lemma 3: Use associative property in the third term
+lemma AddAux3(x: string, y: string, oldSb: string, sb: string, oldI: int,
+              oldJ: int, i:int, j:int, carry:nat, bitX:nat, bitY:nat, digit:nat, sum:nat, oldCarry:nat)
+  requires AddAuxPred(x, y, oldSb, sb, oldI, oldJ, i, j, carry, bitX, bitY, digit, sum, oldCarry)
+  ensures Str2Int(oldSb) +
+          (oldCarry * Pow2(|oldSb|)) +
+          (if oldI >= 0 then (Str2Int(x[0..oldI]) * 2) * Pow2(|oldSb|) + bitX * Pow2(|oldSb|) else 0) +
+          (if oldJ >= 0 then (Str2Int(y[0..oldJ]) * 2 + bitY) * Pow2(|oldSb|) else 0) ==
+          Str2Int(oldSb) +
+          (oldCarry * Pow2(|oldSb|)) +
+          (if oldI >= 0 then Str2Int(x[0..oldI]) * (2 * Pow2(|oldSb|)) + bitX * Pow2(|oldSb|) else 0) +
+          (if oldJ >= 0 then (Str2Int(y[0..oldJ]) * 2 + bitY) * Pow2(|oldSb|) else 0)
+{
+  if oldI >= 0 {
+    assert (Str2Int(x[0..oldI]) * 2) * Pow2(|oldSb|) == Str2Int(x[0..oldI]) * (2 * Pow2(|oldSb|)) by {
+      MulIsAssociative(Str2Int(x[0..oldI]), 2, Pow2(|oldSb|));
+    }
+  }
+}
+
+// Lemma 4: Apply identity: 2 * Pow2(n) = Pow2(n+1) in the third term
+lemma AddAux4(x: string, y: string, oldSb: string, sb: string, oldI: int,
+              oldJ: int, i:int, j:int, carry:nat, bitX:nat, bitY:nat, digit:nat, sum:nat, oldCarry:nat)
+  requires AddAuxPred(x, y, oldSb, sb, oldI, oldJ, i, j, carry, bitX, bitY, digit, sum, oldCarry)
+  ensures Str2Int(oldSb) +
+          (oldCarry * Pow2(|oldSb|)) +
+          (if oldI >= 0 then Str2Int(x[0..oldI]) * (2 * Pow2(|oldSb|)) + bitX * Pow2(|oldSb|) else 0) +
+          (if oldJ >= 0 then (Str2Int(y[0..oldJ]) * 2 + bitY) * Pow2(|oldSb|) else 0) ==
+          Str2Int(oldSb) +
+          (oldCarry * Pow2(|oldSb|)) +
+          (if oldI >= 0 then Str2Int(x[0..oldI]) * Pow2(|oldSb| + 1) + bitX * Pow2(|oldSb|) else 0) +
+          (if oldJ >= 0 then (Str2Int(y[0..oldJ]) * 2 + bitY) * Pow2(|oldSb|) else 0)
+{
+  assert Pow2(|oldSb| + 1) == 2 * Pow2(|oldSb|) by {
+    Pow2Inductive(|oldSb|);
+  }
+}
+
+// Lemma 5: Start distributing Pow2(|oldSb|) in the fourth term
+lemma AddAux5(x: string, y: string, oldSb: string, sb: string, oldI: int,
+              oldJ: int, i:int, j:int, carry:nat, bitX:nat, bitY:nat, digit:nat, sum:nat, oldCarry:nat)
+  requires AddAuxPred(x, y, oldSb, sb, oldI, oldJ, i, j, carry, bitX, bitY, digit, sum, oldCarry)
+  ensures Str2Int(oldSb) +
+          (oldCarry * Pow2(|oldSb|)) +
+          (if oldI >= 0 then Str2Int(x[0..oldI]) * Pow2(|oldSb| + 1) + bitX * Pow2(|oldSb|) else 0) +
+          (if oldJ >= 0 then (Str2Int(y[0..oldJ]) * 2 + bitY) * Pow2(|oldSb|) else 0) ==
+          Str2Int(oldSb) +
+          (oldCarry * Pow2(|oldSb|)) +
+          (if oldI >= 0 then Str2Int(x[0..oldI]) * Pow2(|oldSb| + 1) + bitX * Pow2(|oldSb|) else 0) +
+          (if oldJ >= 0 then (Str2Int(y[0..oldJ]) * 2) * Pow2(|oldSb|) + bitY * Pow2(|oldSb|) else 0)
+{
+  if oldJ >= 0 {
+    var A := Str2Int(y[0..oldJ]);
+    var B := bitY;
+    var C := Pow2(|oldSb|);
+    Rearrange(A, B, C);
+  }
+}
+
+// Lemma 6: Use associative property in the fourth term
+lemma AddAux6(x: string, y: string, oldSb: string, sb: string, oldI: int,
+              oldJ: int, i:int, j:int, carry:nat, bitX:nat, bitY:nat, digit:nat, sum:nat, oldCarry:nat)
+  requires AddAuxPred(x, y, oldSb, sb, oldI, oldJ, i, j, carry, bitX, bitY, digit, sum, oldCarry)
+  ensures Str2Int(oldSb) +
+          (oldCarry * Pow2(|oldSb|)) +
+          (if oldI >= 0 then Str2Int(x[0..oldI]) * Pow2(|oldSb| + 1) + bitX * Pow2(|oldSb|) else 0) +
+          (if oldJ >= 0 then (Str2Int(y[0..oldJ]) * 2) * Pow2(|oldSb|) + bitY * Pow2(|oldSb|) else 0) ==
+          Str2Int(oldSb) +
+          (oldCarry * Pow2(|oldSb|)) +
+          (if oldI >= 0 then Str2Int(x[0..oldI]) * Pow2(|oldSb| + 1) + bitX * Pow2(|oldSb|) else 0) +
+          (if oldJ >= 0 then Str2Int(y[0..oldJ]) * (2 * Pow2(|oldSb|)) + bitY * Pow2(|oldSb|) else 0)
+{
+  if oldJ >= 0 {
+    assert (Str2Int(y[0..oldJ]) * 2) * Pow2(|oldSb|) == Str2Int(y[0..oldJ]) * (2 * Pow2(|oldSb|)) by {
+      MulIsAssociative(Str2Int(y[0..oldJ]), 2, Pow2(|oldSb|));
+    }
+  }
+}
+
+// Lemma 7: Apply identity: 2 * Pow2(n) = Pow2(n+1) in the fourth term
+lemma AddAux7(x: string, y: string, oldSb: string, sb: string, oldI: int,
+              oldJ: int, i:int, j:int, carry:nat, bitX:nat, bitY:nat, digit:nat, sum:nat, oldCarry:nat)
+  requires AddAuxPred(x, y, oldSb, sb, oldI, oldJ, i, j, carry, bitX, bitY, digit, sum, oldCarry)
+  ensures Str2Int(oldSb) +
+          (oldCarry * Pow2(|oldSb|)) +
+          (if oldI >= 0 then Str2Int(x[0..oldI]) * Pow2(|oldSb| + 1) + bitX * Pow2(|oldSb|) else 0) +
+          (if oldJ >= 0 then Str2Int(y[0..oldJ]) * (2 * Pow2(|oldSb|)) + bitY * Pow2(|oldSb|) else 0) ==
+          Str2Int(oldSb) +
+          (oldCarry * Pow2(|oldSb|)) +
+          (if oldI >= 0 then Str2Int(x[0..oldI]) * Pow2(|oldSb| + 1) + bitX * Pow2(|oldSb|) else 0) +
+          (if oldJ >= 0 then Str2Int(y[0..oldJ]) * Pow2(|oldSb| + 1) + bitY * Pow2(|oldSb|) else 0)
+{
+  Pow2Inductive(|oldSb|);
+}
+
+// Lemma 8: Rearrange terms
+lemma AddAux8(x: string, y: string, oldSb: string, sb: string, oldI: int,
+              oldJ: int, i:int, j:int, carry:nat, bitX:nat, bitY:nat, digit:nat, sum:nat, oldCarry:nat)
+  requires AddAuxPred(x, y, oldSb, sb, oldI, oldJ, i, j, carry, bitX, bitY, digit, sum, oldCarry)
+  ensures Str2Int(oldSb) +
+          (oldCarry * Pow2(|oldSb|)) +
+          (if oldI >= 0 then Str2Int(x[0..oldI]) * Pow2(|oldSb| + 1) + bitX * Pow2(|oldSb|) else 0) +
+          (if oldJ >= 0 then Str2Int(y[0..oldJ]) * Pow2(|oldSb| + 1) + bitY * Pow2(|oldSb|) else 0) ==
+          Str2Int(oldSb) +
+          ((oldCarry * Pow2(|oldSb|)) +
+           (if oldI >= 0 then bitX else 0) * Pow2(|oldSb|)) + (if oldJ >= 0 then bitY else 0) * Pow2(|oldSb|) +
+          (if oldI >= 0 then Str2Int(x[0..oldI]) * Pow2(|oldSb| + 1) else 0) +
+          (if oldJ >= 0 then Str2Int(y[0..oldJ]) * Pow2(|oldSb| + 1) else 0)
+{
+  // Simple rearrangement of terms
+}
+
+// Lemma 9: Group bit terms
+lemma AddAux9(x: string, y: string, oldSb: string, sb: string, oldI: int,
+              oldJ: int, i:int, j:int, carry:nat, bitX:nat, bitY:nat, digit:nat, sum:nat, oldCarry:nat)
+  requires AddAuxPred(x, y, oldSb, sb, oldI, oldJ, i, j, carry, bitX, bitY, digit, sum, oldCarry)
+  ensures Str2Int(oldSb) +
+          ((oldCarry * Pow2(|oldSb|)) +
+           (if oldI >= 0 then bitX else 0) * Pow2(|oldSb|)) + (if oldJ >= 0 then bitY else 0) * Pow2(|oldSb|) +
+          (if oldI >= 0 then Str2Int(x[0..oldI]) * Pow2(|oldSb| + 1) else 0) +
+          (if oldJ >= 0 then Str2Int(y[0..oldJ]) * Pow2(|oldSb| + 1) else 0) ==
+          Str2Int(oldSb) +
+          ((oldCarry + (if oldI >= 0 then bitX else 0) + (if oldJ >= 0 then bitY else 0)) * Pow2(|oldSb|)) +
+          (if oldI >= 0 then Str2Int(x[0..oldI]) * Pow2(|oldSb| + 1) else 0) +
+          (if oldJ >= 0 then Str2Int(y[0..oldJ]) * Pow2(|oldSb| + 1) else 0)
+{
+  // Grouping terms with the same factor Pow2(|oldSb|)
+}
+
+// Lemma 10: By definition of sum in the code
+lemma AddAux10(x: string, y: string, oldSb: string, sb: string, oldI: int,
+               oldJ: int, i:int, j:int, carry:nat, bitX:nat, bitY:nat, digit:nat, sum:nat, oldCarry:nat)
+  requires AddAuxPred(x, y, oldSb, sb, oldI, oldJ, i, j, carry, bitX, bitY, digit, sum, oldCarry)
+  ensures Str2Int(oldSb) +
+          ((oldCarry + (if oldI >= 0 then bitX else 0) + (if oldJ >= 0 then bitY else 0)) * Pow2(|oldSb|)) +
+          (if oldI >= 0 then Str2Int(x[0..oldI]) * Pow2(|oldSb| + 1) else 0) +
+          (if oldJ >= 0 then Str2Int(y[0..oldJ]) * Pow2(|oldSb| + 1) else 0) ==
+          Str2Int(oldSb) +
+          (sum * Pow2(|oldSb|)) +
+          (if oldI >= 0 then Str2Int(x[0..oldI]) * Pow2(|oldSb| + 1) else 0) +
+          (if oldJ >= 0 then Str2Int(y[0..oldJ]) * Pow2(|oldSb| + 1) else 0)
+{
+  assert oldCarry + (if oldI >= 0 then bitX else 0) + (if oldJ >= 0 then bitY else 0) == sum;
+}
+
+// Lemma 11: sum = 2*carry + digit
+lemma AddAux11(x: string, y: string, oldSb: string, sb: string, oldI: int,
+               oldJ: int, i:int, j:int, carry:nat, bitX:nat, bitY:nat, digit:nat, sum:nat, oldCarry:nat)
+  requires AddAuxPred(x, y, oldSb, sb, oldI, oldJ, i, j, carry, bitX, bitY, digit, sum, oldCarry)
+  ensures Str2Int(oldSb) +
+          (sum * Pow2(|oldSb|)) +
+          (if oldI >= 0 then Str2Int(x[0..oldI]) * Pow2(|oldSb| + 1) else 0) +
+          (if oldJ >= 0 then Str2Int(y[0..oldJ]) * Pow2(|oldSb| + 1) else 0) ==
+          Str2Int(oldSb) +
+          ((2 * carry + digit) * Pow2(|oldSb|)) +
+          (if oldI >= 0 then Str2Int(x[0..oldI]) * Pow2(|oldSb| + 1) else 0) +
+          (if oldJ >= 0 then Str2Int(y[0..oldJ]) * Pow2(|oldSb| + 1) else 0)
+{
+  assert sum == 2 * carry + digit by {
+    assert carry == sum / 2;
+    assert digit == sum % 2;
+    assert sum == (sum / 2) * 2 + (sum % 2);
+  }
+}
+
+// Lemma 12: Distribute Pow2(|oldSb|)
+lemma AddAux12(x: string, y: string, oldSb: string, sb: string, oldI: int,
+               oldJ: int, i:int, j:int, carry:nat, bitX:nat, bitY:nat, digit:nat, sum:nat, oldCarry:nat)
+  requires AddAuxPred(x, y, oldSb, sb, oldI, oldJ, i, j, carry, bitX, bitY, digit, sum, oldCarry)
+  ensures Str2Int(oldSb) +
+          ((2 * carry + digit) * Pow2(|oldSb|)) +
+          (if oldI >= 0 then Str2Int(x[0..oldI]) * Pow2(|oldSb| + 1) else 0) +
+          (if oldJ >= 0 then Str2Int(y[0..oldJ]) * Pow2(|oldSb| + 1) else 0) ==
+          Str2Int(oldSb) +
+          (digit * Pow2(|oldSb|)) +
+          (carry * Pow2(|oldSb| + 1)) +
+          (if oldI >= 0 then Str2Int(x[0..oldI]) * Pow2(|oldSb| + 1) else 0) +
+          (if oldJ >= 0 then Str2Int(y[0..oldJ]) * Pow2(|oldSb| + 1) else 0)
+{
+  calc {
+    ((2 * carry + digit) * Pow2(|oldSb|));
+  ==
+    2 * carry * Pow2(|oldSb|) + digit * Pow2(|oldSb|);
+  ==
+    {
+      Pow2Inductive(|oldSb|);
+    }
+    (digit * Pow2(|oldSb|)) + (carry * Pow2(|oldSb| + 1));
+  }
+}
+
+// Lemma 13: Definition of Str2Int for new digit + oldSb
+lemma AddAux13(x: string, y: string, oldSb: string, sb: string, oldI: int,
+               oldJ: int, i:int, j:int, carry:nat, bitX:nat, bitY:nat, digit:nat, sum:nat, oldCarry:nat)
+  requires AddAuxPred(x, y, oldSb, sb, oldI, oldJ, i, j, carry, bitX, bitY, digit, sum, oldCarry)
+  ensures Str2Int(oldSb) +
+          (digit * Pow2(|oldSb|)) +
+          (carry * Pow2(|oldSb| + 1)) +
+          (if oldI >= 0 then Str2Int(x[0..oldI]) * Pow2(|oldSb| + 1) else 0) +
+          (if oldJ >= 0 then Str2Int(y[0..oldJ]) * Pow2(|oldSb| + 1) else 0) ==
+          Str2Int(if digit == 1 then ['1'] + oldSb else ['0'] + oldSb) +
+          (carry * Pow2(|oldSb| + 1)) +
+          (if oldI - 1 >= 0 then Str2Int(x[0..(oldI-1)+1]) * Pow2(|oldSb| + 1) else 0) +
+          (if oldJ - 1 >= 0 then Str2Int(y[0..(oldJ-1)+1]) * Pow2(|oldSb| + 1) else 0)
+{
+  PrependDigitToString(digit, oldSb);
+}
+
+// Lemma 14: By definition of sb and updated i, j
+lemma AddAux14(x: string, y: string, oldSb: string, sb: string, oldI: int,
+               oldJ: int, i:int, j:int, carry:nat, bitX:nat, bitY:nat, digit:nat, sum:nat, oldCarry:nat)
+  requires AddAuxPred(x, y, oldSb, sb, oldI, oldJ, i, j, carry, bitX, bitY, digit, sum, oldCarry)
+  ensures Str2Int(if digit == 1 then ['1'] + oldSb else ['0'] + oldSb) +
+          (carry * Pow2(|oldSb| + 1)) +
+          (if oldI - 1 >= 0 then Str2Int(x[0..(oldI-1)+1]) * Pow2(|oldSb| + 1) else 0) +
+          (if oldJ - 1 >= 0 then Str2Int(y[0..(oldJ-1)+1]) * Pow2(|oldSb| + 1) else 0) ==
+          Str2Int(sb) +
+          (carry * Pow2(|sb|)) +
+          (if i >= 0 then Str2Int(x[0..i+1]) * Pow2(|sb|) else 0) +
+          (if j >= 0 then Str2Int(y[0..j+1]) * Pow2(|sb|) else 0)
+{
+  assert Pow2(|sb|) == Pow2(|oldSb| + 1);
+  assert (if digit == 1 then ['1'] + oldSb else ['0'] + oldSb) == sb;
+
+  if oldI >= 0 {
+    assert i == oldI - 1;
+    if i >= 0 {
+      assert x[0..i+1] == x[0..oldI];
+    }
+  }
+
+  if oldJ >= 0 {
+    assert j == oldJ - 1;
+    if j >= 0 {
+      assert y[0..j+1] == y[0..oldJ];
+    }
+  }
+}
+
+// Top-level lemma that combines all the individual steps
+lemma AddAuxTop(x: string, y: string, oldSb: string, sb: string, oldI: int,
+                oldJ: int, i:int, j:int, carry:nat, bitX:nat, bitY:nat, digit:nat, sum:nat, oldCarry:nat)
+  requires AddAuxPred(x, y, oldSb, sb, oldI, oldJ, i, j, carry, bitX, bitY, digit, sum, oldCarry)
   ensures Str2Int(oldSb) +
           (oldCarry * Pow2(|oldSb|)) +
           (if oldI >= 0 then Str2Int(x[0..oldI+1]) * Pow2(|oldSb|) else 0) +
@@ -425,141 +702,23 @@ lemma {:isolate_assertions} AddAux(x: string, y: string, oldSb: string, sb: stri
           (if i >= 0 then Str2Int(x[0..i+1]) * Pow2(|sb|) else 0) +
           (if j >= 0 then Str2Int(y[0..j+1]) * Pow2(|sb|) else 0)
 {
-  calc {
-    Str2Int(oldSb) +
-    (oldCarry * Pow2(|oldSb|)) +
-    (if oldI >= 0 then Str2Int(x[0..oldI+1]) * Pow2(|oldSb|) else 0) +
-    (if oldJ >= 0 then Str2Int(y[0..oldJ+1]) * Pow2(|oldSb|) else 0);
-  == // Split the x[0..oldI+1] into x[0..oldI] and the last bit
-    {
-      BitStringDecomposition(x, oldI);
-      BitStringDecomposition(y, oldJ);
-    }
-
-
-
-    Str2Int(oldSb) +
-    (oldCarry * Pow2(|oldSb|)) +
-    (if oldI >= 0 then (Str2Int(x[0..oldI]) * 2 + bitX) * Pow2(|oldSb|) else 0) +
-    (if oldJ >= 0 then (Str2Int(y[0..oldJ]) * 2 + bitY) * Pow2(|oldSb|) else 0);
-
-  == // Start distributing Pow2(|oldSb|) in the third term
-    Str2Int(oldSb) +
-    (oldCarry * Pow2(|oldSb|)) +
-    (if oldI >= 0 then (Str2Int(x[0..oldI]) * 2) * Pow2(|oldSb|) + bitX * Pow2(|oldSb|) else 0) +
-    (if oldJ >= 0 then (Str2Int(y[0..oldJ]) * 2 + bitY) * Pow2(|oldSb|) else 0);
-
-  == // Use associative property: (a * b) * c = a * (b * c) in the third term
-    {
-      if oldI >= 0 {
-        assert (Str2Int(x[0..oldI]) * 2) * Pow2(|oldSb|) == Str2Int(x[0..oldI]) * (2 * Pow2(|oldSb|));
-      }
-    }
-    Str2Int(oldSb) +
-    (oldCarry * Pow2(|oldSb|)) +
-    (if oldI >= 0 then Str2Int(x[0..oldI]) * (2 * Pow2(|oldSb|)) + bitX * Pow2(|oldSb|) else 0) +
-    (if oldJ >= 0 then (Str2Int(y[0..oldJ]) * 2 + bitY) * Pow2(|oldSb|) else 0);
-
-  == // Apply identity: 2 * Pow2(n) = Pow2(n+1) in the third term
-    {
-      assert Pow2(|oldSb| + 1) == 2 * Pow2(|oldSb|) by {
-        Pow2Inductive(|oldSb|);
-      }
-    }
-    Str2Int(oldSb) +
-    (oldCarry * Pow2(|oldSb|)) +
-    (if oldI >= 0 then Str2Int(x[0..oldI]) * Pow2(|oldSb| + 1) + bitX * Pow2(|oldSb|) else 0) +
-    (if oldJ >= 0 then (Str2Int(y[0..oldJ]) * 2 + bitY) * Pow2(|oldSb|) else 0);
-
-  == // Start distributing Pow2(|oldSb|) in the fourth term
-    Str2Int(oldSb) +
-    (oldCarry * Pow2(|oldSb|)) +
-    (if oldI >= 0 then Str2Int(x[0..oldI]) * Pow2(|oldSb| + 1) + bitX * Pow2(|oldSb|) else 0) +
-    (if oldJ >= 0 then (Str2Int(y[0..oldJ]) * 2) * Pow2(|oldSb|) + bitY * Pow2(|oldSb|) else 0);
-
-  == // Use associative property in the fourth term
-    {
-      if oldJ >= 0 {
-        assert (Str2Int(y[0..oldJ]) * 2) * Pow2(|oldSb|) == Str2Int(y[0..oldJ]) * (2 * Pow2(|oldSb|));
-      }
-    }
-    Str2Int(oldSb) +
-    (oldCarry * Pow2(|oldSb|)) +
-    (if oldI >= 0 then Str2Int(x[0..oldI]) * Pow2(|oldSb| + 1) + bitX * Pow2(|oldSb|) else 0) +
-    (if oldJ >= 0 then Str2Int(y[0..oldJ]) * (2 * Pow2(|oldSb|)) + bitY * Pow2(|oldSb|) else 0);
-
-  == // Apply identity: 2 * Pow2(n) = Pow2(n+1) in the fourth term
-    {
-      Pow2Inductive(|oldSb|);
-    }
-    Str2Int(oldSb) +
-    (oldCarry * Pow2(|oldSb|)) +
-    (if oldI >= 0 then Str2Int(x[0..oldI]) * Pow2(|oldSb| + 1) + bitX * Pow2(|oldSb|) else 0) +
-    (if oldJ >= 0 then Str2Int(y[0..oldJ]) * Pow2(|oldSb| + 1) + bitY * Pow2(|oldSb|) else 0);
-  ==
-    Str2Int(oldSb) +
-    ((oldCarry * Pow2(|oldSb|)) +
-     (if oldI >= 0 then bitX else 0) * Pow2(|oldSb|)) + (if oldJ >= 0 then bitY else 0) * Pow2(|oldSb|) +
-    (if oldI >= 0 then Str2Int(x[0..oldI]) * Pow2(|oldSb| + 1) else 0) +
-    (if oldJ >= 0 then Str2Int(y[0..oldJ]) * Pow2(|oldSb| + 1) else 0);
-  ==
-    Str2Int(oldSb) +
-    ((oldCarry * Pow2(|oldSb|)) + ((if oldI >= 0 then bitX else 0) + (if oldJ >= 0 then bitY else 0)) * Pow2(|oldSb|)) +
-    (if oldI >= 0 then Str2Int(x[0..oldI]) * Pow2(|oldSb| + 1) else 0) +
-    (if oldJ >= 0 then Str2Int(y[0..oldJ]) * Pow2(|oldSb| + 1) else 0);
-  == // Group bitX, bitY and oldCarry terms
-    Str2Int(oldSb) +
-    ((oldCarry + (if oldI >= 0 then bitX else 0) + (if oldJ >= 0 then bitY else 0)) * Pow2(|oldSb|)) +
-    (if oldI >= 0 then Str2Int(x[0..oldI]) * Pow2(|oldSb| + 1) else 0) +
-    (if oldJ >= 0 then Str2Int(y[0..oldJ]) * Pow2(|oldSb| + 1) else 0);
-  == // By definition of sum in the code
-    {
-      assert oldCarry + (if oldI >= 0 then bitX else 0) + (if oldJ >= 0 then bitY else 0) == sum;
-    }
-    Str2Int(oldSb) +
-    (sum * Pow2(|oldSb|)) +
-    (if oldI >= 0 then Str2Int(x[0..oldI]) * Pow2(|oldSb| + 1) else 0) +
-    (if oldJ >= 0 then Str2Int(y[0..oldJ]) * Pow2(|oldSb| + 1) else 0);
-  == // sum = 2*carry + digit
-    Str2Int(oldSb) +
-    ((2 * carry + digit) * Pow2(|oldSb|)) +
-    (if oldI >= 0 then Str2Int(x[0..oldI]) * Pow2(|oldSb| + 1) else 0) +
-    (if oldJ >= 0 then Str2Int(y[0..oldJ]) * Pow2(|oldSb| + 1) else 0);
-  == // Distribute Pow2(|oldSb|)
-    {
-      calc {
-        ((2 * carry + digit) * Pow2(|oldSb|));
-        2 * carry * Pow2(|oldSb|) + digit * Pow2(|oldSb|);
-        {
-          Pow2Inductive(|oldSb|);
-        }
-        (digit * Pow2(|oldSb|)) + (carry * Pow2(|oldSb| + 1));
-      }
-    }
-    Str2Int(oldSb) +
-    (digit * Pow2(|oldSb|)) +
-    (carry * Pow2(|oldSb| + 1)) +
-    (if oldI >= 0 then Str2Int(x[0..oldI]) * Pow2(|oldSb| + 1) else 0) +
-    (if oldJ >= 0 then Str2Int(y[0..oldJ]) * Pow2(|oldSb| + 1) else 0);
-  == // Definition of Str2Int for new digit + oldSb
-    {
-      PrependDigitToString(digit, oldSb);
-    }
-    Str2Int(if digit == 1 then ['1'] + oldSb else ['0'] + oldSb) +
-    (carry * Pow2(|oldSb| + 1)) +
-    (if oldI - 1 >= 0 then Str2Int(x[0..(oldI-1)+1]) * Pow2(|oldSb| + 1) else 0) +
-    (if oldJ - 1 >= 0 then Str2Int(y[0..(oldJ-1)+1]) * Pow2(|oldSb| + 1) else 0);
-  == // By definition of sb and updated i, j
-    {
-      assert Pow2(|sb|) == Pow2(|oldSb| + 1);
-      assert (if digit == 1 then ['1'] + oldSb else ['0'] + oldSb) == sb;
-    }
-    Str2Int(sb) +
-    (carry * Pow2(|sb|)) +
-    (if i >= 0 then Str2Int(x[0..i+1]) * Pow2(|sb|) else 0) +
-    (if j >= 0 then Str2Int(y[0..j+1]) * Pow2(|sb|) else 0);
-  }
+  // Call all the sub-lemmas in sequence to establish the proof
+  AddAux1(x, y, oldSb, sb, oldI, oldJ, i, j, carry, bitX, bitY, digit, sum, oldCarry);
+  AddAux2(x, y, oldSb, sb, oldI, oldJ, i, j, carry, bitX, bitY, digit, sum, oldCarry);
+  AddAux3(x, y, oldSb, sb, oldI, oldJ, i, j, carry, bitX, bitY, digit, sum, oldCarry);
+  AddAux4(x, y, oldSb, sb, oldI, oldJ, i, j, carry, bitX, bitY, digit, sum, oldCarry);
+  AddAux5(x, y, oldSb, sb, oldI, oldJ, i, j, carry, bitX, bitY, digit, sum, oldCarry);
+  AddAux6(x, y, oldSb, sb, oldI, oldJ, i, j, carry, bitX, bitY, digit, sum, oldCarry);
+  AddAux7(x, y, oldSb, sb, oldI, oldJ, i, j, carry, bitX, bitY, digit, sum, oldCarry);
+  AddAux8(x, y, oldSb, sb, oldI, oldJ, i, j, carry, bitX, bitY, digit, sum, oldCarry);
+  AddAux9(x, y, oldSb, sb, oldI, oldJ, i, j, carry, bitX, bitY, digit, sum, oldCarry);
+  AddAux10(x, y, oldSb, sb, oldI, oldJ, i, j, carry, bitX, bitY, digit, sum, oldCarry);
+  AddAux11(x, y, oldSb, sb, oldI, oldJ, i, j, carry, bitX, bitY, digit, sum, oldCarry);
+  AddAux12(x, y, oldSb, sb, oldI, oldJ, i, j, carry, bitX, bitY, digit, sum, oldCarry);
+  AddAux13(x, y, oldSb, sb, oldI, oldJ, i, j, carry, bitX, bitY, digit, sum, oldCarry);
+  AddAux14(x, y, oldSb, sb, oldI, oldJ, i, j, carry, bitX, bitY, digit, sum, oldCarry);
 }
+
 
 predicate SubAuxPred(x: string, y: string, oldSb: string, sb: string, oldI: int,
                      oldJ: int, i:int, j:int, borrow:nat, bitX:nat, bitY:nat, rawDiff:int, diff:nat, oldBorrow:nat)
@@ -904,10 +1063,8 @@ method Add(s1: string, s2: string) returns (res: string)
     if i >= 0 { i := i - 1; }
     if j >= 0 { j := j - 1; }
 
-    AddAux(x, y, oldSb, sb, oldI,
-           oldJ, i, j, carry, bitX, bitY, digit, sum, oldCarry);
-
-
+    AddAuxTop(x, y, oldSb, sb, oldI,
+              oldJ, i, j, carry, bitX, bitY, digit, sum, oldCarry);
   }
 
   assert Str2Int(x) + Str2Int(y) == Str2Int(sb);
